Trochę walki z głębokimi regułami indukcji (albo regułami głębokiej indukcji, jak kto woli), ale dość niesukcesowo.

code/IndRec/Typy/Nested/Bush.v
@@ -8,8 +8,22 @@ Inductive BushF (F : Type -> Type) (A : Type) : Type :=
 Fail Inductive Bush (A : Type) : Type :=
     | In : BushF Bush A -> Bush A.
 
+Definition ListC (A : Type) : Type :=
+  forall (R : Type) (nil : R) (cons : A -> R -> R), R.
+
 Definition BushC (A : Type) : Type :=
-  forall (F : Type -> Type) (R : Type) (leaf : F R) (node : A -> F (F R) -> F R), F R.
+  forall (F : Type -> Type) (R : Type) (leaf : R) (node : A -> F R -> R), R.
+
+Definition leaf {A : Type} : BushC A :=
+  fun F R leaf node => leaf.
+
+Definition node {A : Type} (x : A) (b : BushC (BushC A)) : BushC A.
+Proof.
+  unfold BushC.
+  intros F R leaf node.
+  apply (node x).
+  unfold BushC in b.
+Abort.
 
 Definition mapC {A B : Type} (f : A -> B) (b : BushC A) : BushC B.
 Proof.
@@ -20,7 +34,7 @@ Proof.
     exact leaf.
     intros a ffr. apply node.
       apply f. exact a.
-      exact ffr. Show Proof.
+      exact ffr.
 Defined.
 
 Unset Positivity Checking.
@@ -78,3 +92,106 @@ end.
 Compute  (replicate 3 (Node 5 Leaf)).
 
 Set Guard Checking.
+
+Require Import FunctionalExtensionality.
+
+Print Bush.
+Unset Positivity Checking.
+Inductive Bush' {A : Type} (P : A -> Type) : Bush A -> Type :=
+    | Leaf' : Bush' P Leaf
+    | Node' : forall (x : A) (b : Bush (Bush A)),
+                P x -> Bush' (Bush' P) b -> Bush' P (Node x b).
+Set Positivity Checking.
+
+Fixpoint Bush_ind_deep
+  (P : forall (A : Type) (Q : A -> Type), Bush A -> Type)
+  (leaf : forall (A : Type) (Q : A -> Type), P A Q Leaf)
+  (node : forall (A : Type) (Q : A -> Type) (x : A) (b : Bush (Bush A)),
+            Q x -> P (Bush A) (Bush' Q (*P A Q*)) b -> P A Q (Node x b))
+  {A : Type} (Q : A -> Type)
+  {b : Bush A} (b' : Bush' Q b) {struct b'} : P A Q b.
+Proof.
+  destruct b' as [| x b Qx Pb].
+    apply leaf.
+    apply node.
+      exact Qx.
+      apply Bush_ind_deep; try assumption.
+Defined.
+
+Fixpoint Bush_ind
+  (P : forall (A : Type), Bush A -> Type)
+  (leaf : forall (A : Type), P A Leaf)
+  (node : forall (A : Type) (x : A) (b : Bush (Bush A)),
+            P (Bush A) b -> P A (Node x b))
+  {A : Type}
+  {b : Bush A} {struct b} : P A b.
+Proof.
+  refine (@Bush_ind_deep (fun A _ => P A) _ _ A (fun _ => True) b _); intros.
+    apply leaf.
+    apply node. assumption.
+    admit.
+Admitted.
+
+(*
+Fixpoint Bush_ind_deep'
+  (P : forall (A : Type) (Q : A -> Type), Bush A -> Type)
+  (leaf : forall (A : Type) (Q : A -> Type), P A Q Leaf)
+  (node : forall (A : Type) (Q : A -> Type) (x : A) (b : Bush (Bush A)),
+            Q x -> P (Bush A) (P A Q) b -> P A Q (Node x b))
+  {A : Type} (Q : A -> Type)
+  {b : Bush A} (b' : Bush' Q b) {struct b'} : P A Q b.
+Proof.
+  destruct b' as [| x b Qx Pb].
+    apply leaf.
+    apply node.
+      exact Qx.
+      apply Bush_ind_deep'; try assumption. revert P Q leaf node Qx b Pb. fix IH 6.
+        destruct 4; constructor.
+          apply Bush_ind_deep'; assumption.
+          apply (IH (fun A Q => . assumption.
+Defined.
+*)
+
+Fixpoint Bush_ind_deep''
+  {A : Type} (Q : A -> Type) (P : Bush A -> Type)
+  (leaf : P Leaf)
+  (node : forall (x : A) (b : Bush (Bush A)),
+            Q x -> Bush' P b -> P (Node x b))
+  {b : Bush A} (b' : Bush' Q b) {struct b'} : P b.
+Proof.
+  destruct b' as [| x b Qx Pb].
+    apply leaf.
+    apply node.
+      exact Qx.
+      revert P Q leaf node Qx b Pb. fix IH 6; intros.
+        destruct Pb; constructor.
+          apply (Bush_ind_deep'' A Q P); assumption.
+Abort.
+
+
+
+
+
+
+
+
+
+
+Lemma map_map :
+  forall {A B C : Type} (f : A -> B) (g : B -> C) (b : Bush A),
+    map g (map f b) = map (fun x => g (f x)) b.
+Proof.
+  intro.
+  pose (P := (fun (A : Type) (b : Bush A) => forall (B C : Type) (f : A -> B) (g : B -> C), map g (map f b) = map (fun x => g (f x)) b)).
+  intros B C f g b. revert B C f g.
+  refine (Bush_ind P _ _).
+    unfold P; cbn; intros. reflexivity.
+    unfold P; cbn; intros. f_equal. rewrite !H. f_equal.
+      extensionality bb. rewrite H.
+  
+  fix IH 6.
+  destruct b as [| v bs]; cbn.
+    reflexivity.
+    f_equal. rewrite IH. f_equal.
+      extensionality x. rewrite IH. reflexivity.
+Qed.
